fixes related to communications. Added a test harness for communication test.fs

ModularEngine/src/LogicEngine.FStar/test.fs
@@ -1,0 +1,30 @@
+module Test
+
+exception Error of string
+
+let sendMsg (p:string) (msg:string) =
+  let bytes = System.Text.Encoding.Unicode.GetBytes msg in
+  Net.send p bytes
+
+let getMsg() =
+  let bytes = Net.receive() in
+  let msg = System.Text.Encoding.Unicode.GetString(bytes) in
+  System.Console.WriteLine(msg)
+
+let _ = 
+  let args = System.Environment.GetCommandLineArgs() |> Seq.toList in
+  match args with
+    | [_;configFile] ->
+      if not (System.IO.File.Exists (configFile)) then
+        (System.Console.WriteLine("File not found: {0}", configFile); exit(1))
+      else Authenticate.readConfig configFile
+    | _ -> (System.Console.WriteLine("usage: test config-file-name"); exit(1)) in
+  let p = Authenticate.lookup_me() in
+  if (p = "org1") then sendMsg "site1" "sending from org1 to site1"
+  else if (p = "site1") then
+    (getMsg(); sendMsg "phys1" "sending from site1 to phys1")
+  else if (p = "phys1") then
+    (getMsg(); sendMsg "keyMgr" "sending from phys1 to keyMgr"; getMsg())
+  else if (p = "keyMgr") then
+    (getMsg(); sendMsg "keyMgr" "sending keys from keyMgr to phys1")
+    
