ModularEngine/src/LogicEngine.FStar/state.fst
@@ -5,7 +5,7 @@ private val infos : Ref infostrate
 let infos = newref []
 
 val addToInfostrate : i:infon{Knows i} -> unit
-let addToInfostrate i = infos := i::!infos
+let addToInfostrate i = let _ = infos := i::!infos in ()
 
 val getInfostrate : unit -> infostrate
 let getInfostrate x = !infos
